Fix and tweak final theorem

compilation/proofs/check_countProofScript.sml
@@ -6,12 +6,27 @@ val _ = new_theory"check_countProof";
 
 val check_count_io_events_def = new_specification("check_count_io_events_def",
   ["check_count_io_events","check_count_fs"],
-  check_count_correct |> Q.GENL[`init_out`,`cls`,`fs`] |> Q.SPEC`""`
-  |> SIMP_RULE bool_ss [SKOLEM_THM,GSYM RIGHT_EXISTS_IMP_THM,RIGHT_EXISTS_AND_THM,APPEND]);
+  check_count_correct |> Q.GENL[`init_out`,`cls`,`fs`] |> Q.SPEC`strlit""`
+  |> SIMP_RULE bool_ss [SKOLEM_THM,GSYM RIGHT_EXISTS_IMP_THM,RIGHT_EXISTS_AND_THM,
+                        mlstringTheory.strcat_nil]);
 
 val (check_count_sem,check_count_output) = check_count_io_events_def |> SPEC_ALL |> UNDISCH |> CONJ_PAIR
 val (check_count_not_fail,check_count_sem_sing) =
   MATCH_MP semantics_prog_Terminate_not_Fail check_count_sem |> CONJ_PAIR
+
+val check_count_compiled_def = Define `
+  check_count_compiled = (code,data,config)`;
+
+(* TODO: these are duplicated from wordfreqProof -- they should be elsewhere *)
+val wfFS_def = Define `
+  wfFS fs <=> fsFFIProps$wfFS fs ∧ STD_streams fs ∧ stdout fs (strlit "")`;
+
+val x64_installed_def = Define `
+  x64_installed (c,d,conf) ffi mc ms <=>
+    is_x64_machine_config mc ∧
+    backendProof$installed c d conf.ffi_names ffi
+      (heap_regs x64_backend_config.stack_conf.reg_names) mc ms`
+(* -- *)
 
 val compile_correct_applied =
   MATCH_MP compile_correct check_count_compiled
@@ -24,9 +39,38 @@ val compile_correct_applied =
   |> DISCH(#1(dest_imp(concl x64_init_ok)))
   |> REWRITE_RULE[AND_IMP_INTRO]
 
-val check_count_compiled_thm =
-  CONJ compile_correct_applied check_count_output
-  |> DISCH_ALL
-  |> curry save_thm "check_count_compiled_thm";
+val check_count_compiled_thm = Q.store_thm("check_count_compiled_thm",
+  `check_countProof$wfFS fs ∧
+   x64_installed check_count_compiled (basis_ffi cl fs) mc ms
+   ⇒
+   ∃io_events fs'.
+   machine_sem mc (basis_ffi cl fs) ms ⊆
+   extend_with_resource_limit {Terminate Success io_events} ∧
+   extract_fs fs io_events = SOME fs' ∧
+   (stdout fs' (strlit "Certificate OK\n") ⇔
+    Check_Certificate (lines_of (implode (get_stdin fs))))`,
+  simp[wfFS_def,Once (GSYM AND_IMP_INTRO)]
+  \\ disch_then assume_tac
+  \\ simp[x64_installed_def,check_count_compiled_def]
+  \\ disch_then assume_tac
+  \\ qmatch_asmsub_rename_tac`basis_ffi cls`
+  \\ assume_tac (UNDISCH compile_correct_applied)
+  \\ asm_exists_tac
+  \\ simp[check_count_output]
+  \\ `∃inp pos. stdin fs inp pos`
+  by (
+    fs[TextIOProofTheory.stdin_def,
+       fsFFIPropsTheory.STD_streams_def,
+       fsFFIPropsTheory.wfFS_def]
+    \\ last_assum(qspecl_then[`0`,`inp`]mp_tac)
+    \\ simp_tac std_ss [] \\ strip_tac
+    \\ imp_res_tac ALOOKUP_MEM
+    \\ last_x_assum(qspec_then`0`mp_tac)
+    \\ simp[MEM_MAP,EXISTS_PROD]
+    \\ Cases_on`ALOOKUP fs.files (IOStream (strlit"stdin"))` \\ fs[]
+    \\ fs[ALOOKUP_FAILS]
+    \\ metis_tac[] )
+  \\ simp[UNDISCH (GSYM TextIOProofTheory.linesFD_splitlines_get_stdin)]
+  \\ simp[fsFFIPropsTheory.lines_of_def,MAP_MAP_o,o_DEF,mlstringTheory.strcat_thm]);
 
 val _ = export_theory();
